\batchmode
\documentclass{article}
\usepackage{ifthen}
\usepackage{epsfig}
\usepackage[utf8]{inputenc}
% Packages requested by user
\usepackage{amsmath}
\usepackage{amssymb}

\usepackage{newunicodechar}
  \newunicodechar{⁻}{${}^{-}$}% Superscript minus
  \newunicodechar{²}{${}^{2}$}% Superscript two
  \newunicodechar{³}{${}^{3}$}% Superscript three

\pagestyle{empty}
\begin{document}
$\Omega$
\pagebreak

$\Omega_h$
\pagebreak

$u_i(\vec{x},t)$
\pagebreak

$u_{h,i}(\vec{x},t)$
\pagebreak

$u_{h,i}$
\pagebreak

$N_{h,i}$
\pagebreak

$N_h = \sum_{i=1}^n N_{h,i}$
\pagebreak

$\mathbb{R}^{N_{h,i}}$
\pagebreak

$\vec{u}_{h,i} \in \mathbb{R}^{N_{h,i}}$
\pagebreak

$(\vec{u}_{h,i})_j \in \mathbb{R}$
\pagebreak

$\vec{u} = \vec{u}_1$
\pagebreak

$\mathcal{M}_h(\cdot)$
\pagebreak

$\mathcal{A}_h(\cdot)$
\pagebreak

$\vec{f_h}$
\pagebreak

$ \mathcal{M}_h, \mathcal{A}_h: \mathbb{R}^{N_h} \mapsto \mathbb{R}^{N_h} $
\pagebreak

$\vec{f_h} \in \mathbb{R}^{N_h}$
\pagebreak

\begin{align*} \partial_t \mathcal{M}_h(\vec{u}_h) + \mathcal{A}_h(\vec{u}_h) = \vec{f_h} \end{align*}
\pagebreak

$ \mathcal{M}_h(\cdot) = 0 $
\pagebreak

$ \mathcal{A}_h(\vec{u}_h) \equiv A_h \cdot \vec{u}_h $
\pagebreak

$A_h \in \mathbb{R}^{N_h \times N_h}$
\pagebreak

$A_h$
\pagebreak

$\vec{f}_h \in \mathbb{R}^{N_h}$
\pagebreak

\begin{align*} A_h \vec{u}_h = \vec{f}_h. \end{align*}
\pagebreak

$\vec{f}_h$
\pagebreak

$ \mathcal{A}_h(\vec{u}_h): \mathbb{R}^{N_h} \mapsto \mathbb{R}^{N_h}$
\pagebreak

\begin{align*} d_h: \mathbb{R}^{N_h} &\mapsto \mathbb{R}^{N_h}\\ \vec{u}_h &\mapsto \vec{d}_h(\vec{u}_h) := \mathcal{A}_h(\vec{u}_h)-\vec{f}_h. \end{align*}
\pagebreak

$\vec{d}_h(u_h) = 0$
\pagebreak

$u_h^0$
\pagebreak

\begin{align*} \vec{c}_{h,k} &:= (J_h(\vec{u}_{h_k}))^{-1} d_h(\vec{u}_{h,k}),\\ \vec{u}_{h,k+1} &:= \vec{u}_{h,k} - \alpha_k \vec{c}_{h,k} \end{align*}
\pagebreak

$\vec{u}_{h,k}$
\pagebreak

$\vec{c}_{h,k}$
\pagebreak

$J_h(\vec{u}_{h_k})$
\pagebreak

$ \alpha_k$
\pagebreak

\begin{align*} J_h(\vec{u}_{h_k}) = \frac{\partial \vec{d}_h(u_h)}{\partial \vec{u}_h} = \frac{\partial \mathcal{A}_h(u_h)}{\partial \vec{u}_h} \end{align*}
\pagebreak

\begin{align*} (J_h(\vec{u}_{h_k}))_{ij} = \frac{\partial (\vec{d}_h(u_h))_i}{\partial (\vec{u}_h)_j} \end{align*}
\pagebreak

\begin{align*} J_h(\vec{u}_{h_k}) = \mathbb{I} \end{align*}
\pagebreak

\begin{align*} J_h(\vec{u}_{h_k}) \vec{c}_{h,k} = \vec{d}_h(\vec{u}_{h_k}). \end{align*}
\pagebreak

$J_h \equiv A_h$
\pagebreak

$J_h(\vec{u}_h)$
\pagebreak

$\vec{u}_h$
\pagebreak

$\vec{d}_h(\vec{u}_h)$
\pagebreak

\begin{align*} \partial_t u(t) &= - f(t, u(t)) \\ u(t_{start}) &= u_0 \end{align*}
\pagebreak

$u: \mathbb{R} \mapsto \mathbb{R}^N$
\pagebreak

$: \mathbb{R} \times \mathbb{R}^N \mapsto \mathbb{R}^N$
\pagebreak

$\{t_0 = t_{start}, t_1, t_2, \ldots \}$
\pagebreak

$\Delta t^k := t_{k} - t_{k-1}$
\pagebreak

$u^{(k)} \approx u(t_k)$
\pagebreak

$u$
\pagebreak

\begin{align*} \sum_{l=0}^{L-1} \left[ s_{m,l} u^{(k-l)} + s_{a,l} f(t^{k-l}, u^{(k-l)}) \right] = 0. \end{align*}
\pagebreak

$L \geq 2$
\pagebreak

$s_{m,l}, s_{a,l} \in \mathbb{R}$
\pagebreak

$u^{(k)}$
\pagebreak

$t_k$
\pagebreak

$u^{(k-l)} (l \geq 1)$
\pagebreak

$\vec{s} := (s_0, s_1, \ldots, s_{L-1})$
\pagebreak

$ u^{k} - u^{k-1} + \Delta t^k f(t^k, u^k) = 0 $
\pagebreak

$L = 2$
\pagebreak

\begin{align*} \vec{s}_a &= (\Delta t^k, 0)\\ \vec{s}_m &= (1, -1) \end{align*}
\pagebreak

$ u^{k} - u^{k-1} + \Delta t^k f(t^{k-1}, u^{k-1}) = 0 $
\pagebreak

\begin{align*} \vec{s}_a &= (0, \Delta t^k)\\ \vec{s}_m &= (1, -1) \end{align*}
\pagebreak

$ u^{k} - u^{k-1} + \frac{1}{2} \Delta t^k f(t^{k}, u^{k}) + \frac{1}{2} \Delta t^k f(t^{k-1}, u^{k-1}) = 0$
\pagebreak

\begin{align*} \vec{s}_a &= (\frac{1}{2} \Delta t^k, \frac{1}{2} \Delta t^k)\\ \vec{s}_m &= (1, -1) \end{align*}
\pagebreak

$\theta$
\pagebreak

$ u^{k} - u^{k-1} + \theta \Delta t^k f(t^{k}, u^{k}) + (1- \theta) \Delta t^k f(t^{k-1}, u^{k-1}) = 0$
\pagebreak

\begin{align*} \vec{s}_a &= (\theta \Delta t^k, (1- \theta)\Delta t^k)\\ \vec{s}_m &= (1, -1) \end{align*}
\pagebreak

$ \theta$
\pagebreak

$ u^{k} - \frac{4}{3}u^{k-1} + \frac{1}{3}u^{k-2} + \frac{2}{3} \Delta t^k f(t^{k}, u^{k}) = 0$
\pagebreak

$L = 3$
\pagebreak

\begin{align*} \vec{s}_a &= (\frac{2}{3} \Delta t^k, 0, 0)\\ \vec{s}_m &= (1, -\frac{4}{3}, \frac{1}{3}) \end{align*}
\pagebreak

$\mathcal{M}(u)$
\pagebreak

$\frac{\partial}{\partial t} u$
\pagebreak

\begin{align*} \mathcal{M}(u) = \frac{\partial}{\partial t} u = - \mathcal{A}(u, t) + f(t) \end{align*}
\pagebreak

\begin{align*} \frac{\partial}{\partial t} M_h \vec{u}_h(t) = - \mathcal{A}_h(\vec{u}_h(t), t) + f_h(t). \end{align*}
\pagebreak

\begin{align*} \vec{d}_h(\vec{u}_h^{(k)}) := \sum_{l=0}^{L-1} \left[ s_{m,l} M_h \vec{u}_h^{(k-l)} + s_{a,l} \left( \mathcal{A}_h(\vec{u}^{(k-l)}, t^{(k-l)}) - \vec{f}_h(t^{(k-l)}) \right) \right] = 0. \end{align*}
\pagebreak

$\vec{d}(u_h^{(k)})$
\pagebreak

\begin{align*} \vec{d}_h(\vec{u}_h^{(k)}) := \sum_{l=0}^{L-1} \hat{\vec{d}}_h(\vec{u}_h^{(k-l)}, t^{(k-l)}, s_{m,l}, s_{a,l}) \end{align*}
\pagebreak

\begin{align*} \hat{\vec{d}}_h(\vec{u}_h, t, s_m, s_a) := s_m M_h \vec{u}_h + s_a \left( \mathcal{A}_h(\vec{u}, t) - \vec{f}_h(t) \right) \end{align*}
\pagebreak

\begin{align*} J_h(\vec{u}_h^{(k)}, t^k, s_{m,0}, s_{a,0}) = \frac{\partial \vec{d}_h(\vec{u}_h)}{\partial \vec{u}_h} \left( \vec{u}_h^{(k)} \right) = \frac{\partial \hat{\vec{d}}_h(\vec{u}_h, t^k, s_{m,0}, s_{a,0})} {\partial \vec{u}_h} \left( \vec{u}_h^{(k)} \right) = s_{m,0} M_h + s_{a,0} \frac{\partial \mathcal{A}_h(\vec{u}_h, t^k)}{\partial \vec{u}_h} \left( \vec{u}_h^{(k)} \right) \end{align*}
\pagebreak

$J_h(\vec{u}_h, t, s_m, s_a)$
\pagebreak

$\vec{u}_h, t, s_m, s_a$
\pagebreak

$\hat{\vec{d}}_h(\vec{u}_h, t, s_m, s_a)$
\pagebreak

$\mathcal{M}(\cdot)$
\pagebreak

$\mathcal{A}(\cdot)$
\pagebreak

$\mathcal{A}(\vec{u}_h) \equiv A_h \vec{u}_h$
\pagebreak

\begin{align*} s_{m,0} M_h \vec{u}_h^{(k)} + s_{a,0} A_h \vec{u}_h^{(k)} = s_{a,0} \vec{f}_h^{(k)} - \sum_{l=1}^{L-1} \left[ s_{m,l} M_h \vec{u}_h^{(k-l)} + s_{a,l} \left( A_h \vec{u}^{(k-l)} - \vec{f}_h^{(k-l)} \right) \right] \end{align*}
\pagebreak

\begin{align*} B_h \vec{u}_h^{(k)} = b_h \end{align*}
\pagebreak

$B_h:=s_{m,0} M_h+ s_{a,0} A_h $
\pagebreak

$b_h:= s_{a,0} \vec{f}_h^{(k)} - \sum_{l=1}^{L-1} \left[ s_{m,l} M_h \vec{u}_h^{(k-l)} + s_{a,l} \left( A_h \vec{u}^{(k-l)} - \vec{f}_h^{(k-l)} \right) \right]$
\pagebreak

\begin{align*} \vec{d}_h(\vec{u}_h^{(k)}) := \sum_{l=0}^{L-1} \left[ s_{m,l} M_h \vec{u}_h^{(k-l)} + s_{a,l} \left( \mathcal{A}_h(\vec{u}^{(k-l)}, t^{(k-l)}) - \vec{f}_h^{(k-l)} \right) \right] = 0 \end{align*}
\pagebreak

$k$
\pagebreak

$ \Omega \subset \mathbb{R}^d $
\pagebreak

$ I := [t_{start}, t_{end}] $
\pagebreak

$ n $
\pagebreak

\begin{align*} u_i : \Omega \times I &\mapsto \mathbb{R}\\ (\vec{x}, t) &\mapsto u_i(\vec{x}, t). \end{align*}
\pagebreak

\begin{align*} \vec{u}(\vec{x},t) := \begin{pmatrix} u_1(\vec{x}, t) \\ \vdots \\ u_n(\vec{x}, t) \end{pmatrix}. \end{align*}
\pagebreak

\begin{align*} \mathcal{M}(\vec{u}) + \mathcal{A}(\vec{u}) &= f, &x\in\Omega,\\ \mathcal{B}(\vec{u}) &= 0, &x\in\partial \Omega. \end{align*}
\pagebreak

\begin{align*} f(\vec{x}, t) &\text{ is a given right - hand side independent of } \vec{u},\\ \mathcal{M} &\text{ is a time-dependent operator acting on } \vec{u},\\ \mathcal{A} &\text{ is a time-independent operator acting in } \vec{u},\\ \mathcal{B} &\text{ are boundary conditions for } \vec{u}. \end{align*}
\pagebreak

$\mathcal{M}$
\pagebreak

$ \mathcal{A}$
\pagebreak

\begin{align*} \partial_t c - \nabla \left( D \nabla c - \vec{v} c \right) + r(c) &= f, &\text{ in } \Omega,\\ c &= g, &\text{ on } \partial\Omega_D,\\ \frac{\partial c}{\partial \vec{n}} &= h &\text{ on } \partial\Omega_N, \end{align*}
\pagebreak

$ c(\vec{x},t)$
\pagebreak

$ D(\vec{x},t)$
\pagebreak

$ v(\vec{x},t)$
\pagebreak

$ r(c, \vec{x},t)$
\pagebreak

$ f(\vec{x},t)$
\pagebreak

$\vec{c}$
\pagebreak

$ \vec{u} = c$
\pagebreak

$ \mathcal{M}(c) := \partial_t c $
\pagebreak

$ \mathcal{A}(c) := - \nabla \left( D \nabla c - \vec{v} c \right) + r(c)$
\pagebreak

$ f = f $
\pagebreak

$ \mathcal{B}(c) := \begin{cases} c(\vec{x}, t) - g(\vec{x}, t), &x \in \partial\Omega_D,\\ \frac{\partial c}{\partial \vec{n}} - h(\vec{x}, t) &x \in \partial\Omega_N. \end{cases}. $
\pagebreak

$ \partial_t c = 0 $
\pagebreak

$ t $
\pagebreak

$ \mathcal{M}(c) = 0 $
\pagebreak

$A_h \left( := \frac{\partial A_h \vec{v}_h}{\partial \vec{v}_h} \left( \vec{u}_h \right) \right)$
\pagebreak

$\vec{d}_h(\vec{u}_h) := A_h \vec{u}_h - \vec{f}_h$
\pagebreak

$J_h(\vec{u}_h) := \frac{\partial \mathcal{A}_h(\vec{v}_h)}{\partial \vec{v}_h} \left( \vec{u}_h \right)$
\pagebreak

$\vec{d}_h(\vec{u}_h) := \mathcal{A}_h(\vec{u}_h)-\vec{f}_h$
\pagebreak

$J_h(\vec{u}_h, s_m, s_a) := s_m M_h + s_a \frac{\partial \mathcal{A}_h(\vec{v}_h)}{\partial \vec{v}_h} \left( \vec{u}_h \right)$
\pagebreak

$\hat{\vec{d}}_h(\vec{u}_h, s_m, s_a) := s_m M_h \vec{u}_h + s_a \mathcal{A}_h(\vec{u}_h)$
\pagebreak

$\mathcal{M}(\vec{u}_h) \equiv M_h \vec{u}_h$
\pagebreak

$\mathcal{A}(\vec{u}_h)$
\pagebreak

$ \frac{\mathcal{M}_h(\vec{v}_h)}{\partial \vec{v}_h} \left( \vec{u}_h \right) \equiv M_h$
\pagebreak

$ \frac{\mathcal{A}_h(\vec{v}_h)}{\partial \vec{v}_h} \left( \vec{u}_h \right) $
\pagebreak

$ N^f $
\pagebreak

$ i \in [0, ..., N^f -1] $
\pagebreak

$ c_0, \ldots, c_4 $
\pagebreak

$i$
\pagebreak

$ c_i $
\pagebreak

$c_2$
\pagebreak

$c_0$
\pagebreak

$n_{sys}$
\pagebreak

\[ \vec{u} = \bigotimes_{s=1}^{n_{sys}} \vec{u}^s \]
\pagebreak

$ I_s $
\pagebreak

$s$
\pagebreak

$ s $
\pagebreak

$ \vec{u}^s$
\pagebreak

$N_s := |I_s|$
\pagebreak

$N := |\bigotimes\limits_{s=1}^{n_{sys}}I_s| = \sum\limits_{s=1}^{n_{sys}} N_s$
\pagebreak

$\vec{u}$
\pagebreak

$N$
\pagebreak

$ \vec{u}^s $
\pagebreak

$ N_s$
\pagebreak

$ i \in I $
\pagebreak

$ \vec{u}_i \in \mathbb{R}$
\pagebreak

$ i \in I_s$
\pagebreak

$ \vec{u}^s_i \in \mathbb{R}$
\pagebreak

$ I $
\pagebreak

$ N $
\pagebreak

\begin{align*} \vec{d}(\vec{u}): \mathbb{R}^N &\mapsto \mathbb{R}^N, \\ J(\vec{u}): \mathbb{R}^N &\mapsto \mathbb{R}^{N \times N}. \end{align*}
\pagebreak

\[ J(\vec{u})_{ij} := \frac{\partial \vec{d}_i}{\partial \vec{u}_j}. \]
\pagebreak

\[ \vec{d}(\vec{u}) = \bigotimes_{s=1}^{n_{sys}} \vec{d}^s(\vec{u}), \]
\pagebreak

\[ J(\vec{u}) = \bigotimes_{s=1}^{n_{sys}} \bigotimes_{t=1}^{n_{sys}} J^{st}(\vec{u}), \]
\pagebreak

\begin{align*} J^{st}(\vec{u}) &:= \frac{\partial \vec{d}^s}{\partial \vec{u}^t},\\ J^{st}(\vec{u})_{ij} &:= \frac{\partial \vec{d}^s_i}{\partial \vec{u}^t_j}. \end{align*}
\pagebreak

$ s$
\pagebreak

$ \vec{u} $
\pagebreak

$ \mathcal{D}$
\pagebreak

$ \mathbb{R}^m$
\pagebreak

\begin{align*} \mathcal{I}: \mathbb{R}^d \times \mathbb{R} \times \mathbb{R}^{N_1} \times \dots \times \mathbb{R}^{N_{n_{sys}}} &\mapsto \mathcal{D} \\ \vec{x}, t, \vec{u}^1, \dots, \vec{u}^{n_{sys}} &\mapsto \mathcal{I}(\vec{x}, t, \vec{u}^1, \dots, \vec{u}^{n_{sys}}) \end{align*}
\pagebreak

\[ \vec{d}^s \equiv \vec{d}^s(\vec{u}^s, \mathcal{I}^s_1, \dots, \mathcal{I}^s_{n_{\mathcal{I}^s}}), \]
\pagebreak

$n_{\mathcal{I}^s}$
\pagebreak

\begin{align*} J^{ss}(\vec{u}) &= \left. \frac{\partial \vec{d}^s}{\partial \vec{u}^s} \right|_{\vec{u}} + \sum_{k=1}^{n_{\mathcal{I}^s}} \left. \frac{\partial \vec{d}^s}{\partial \mathcal{I}^s_k} \right|_{\vec{u}} \cdot \left. \frac{\partial \mathcal{I}^s_k} {\partial \vec{u}^s} \right|_{\vec{u}}\\ J^{st}(\vec{u}) &= \sum_{k=1}^{n_{\mathcal{I}^s}} \left. \frac{\partial \vec{d}^s}{\partial \mathcal{I}^s_k} \right|_{\vec{u}} \cdot \left. \frac{\partial \mathcal{I}^s_k} {\partial \vec{u}^t} \right|_{\vec{u}} \end{align*}
\pagebreak

\begin{align*} \left. \frac{\partial \vec{d}^s}{\partial \vec{u}^s} \right|_{\vec{u}} := \left. \frac{\partial \vec{d}^s(\vec{v}^s, \mathcal{I}^s_1(\vec{u}), \dots, \mathcal{I}^s_{n_{\mathcal{I}^s}}(\vec{u})))} {\partial \vec{v}^s} \right|_{\vec{v}^s = \vec{u}^s} \end{align*}
\pagebreak

\begin{align*} \left. \frac{\partial \vec{d}^s}{\partial \mathcal{I}^s_k} \right|_{\vec{u}} := \left. \frac{\partial \vec{d}^s(\vec{u}^s, \mathcal{I}^s_1(\vec{u}), \dots, \tilde{\mathcal{I}}^s_k, \dots, \mathcal{I}^s_{n_{\mathcal{I}^s}}(\vec{u}))} {\partial \tilde{\mathcal{I}}^s_k} \right|_{\tilde{\mathcal{I}}^s_k = \mathcal{I}^s_k(\vec{u})} \end{align*}
\pagebreak

\begin{align*} \frac{\partial \vec{d}^s_i}{\partial \mathcal{I}^s_k} \end{align*}
\pagebreak

$\mathcal{D}$
\pagebreak

\begin{align*} \left. \frac{\partial \mathcal{I}^s_k} {\partial \vec{u}^t} \right|_{\vec{u}} := \left. \frac{\partial \mathcal{I}^s_k(\vec{u}^1, \dots, \vec{v}^t, \dots, \vec{u}^{n_{sys}})} {\partial \vec{v}^t} \right|_{\vec{v}^t = \vec{u}^t} \end{align*}
\pagebreak

\begin{align*} \frac{\partial \mathcal{I}^s_k}{\partial \vec{u}^t_j} \end{align*}
\pagebreak

\begin{align*} J^{st}(\vec{u})_{ij} = \sum_{k=1}^{n_{\mathcal{I}^s}} \left. \frac{\partial \vec{d}^s_i}{\partial \mathcal{I}^s_k} \right|_{\vec{u}} \cdot \left. \frac{\partial \mathcal{I}^s_k} {\partial \vec{u}^t_j} \right|_{\vec{u}} \end{align*}
\pagebreak

$\mathcal{E}$
\pagebreak

$ \mathcal{E} \equiv \mathcal{E}()$
\pagebreak

$ \mathcal{E} \equiv \mathcal{E}(\vec{x},t)$
\pagebreak

$ \mathcal{E} \equiv \mathcal{E}(\vec{x}, t, \vec{u}^s)$
\pagebreak

$ \mathcal{E} \equiv \mathcal{E}(\vec{x}, t, \vec{u}^1, \dots, \vec{u}^{n_{sys}})$
\pagebreak

\begin{align*} \mathcal{E}: \mathbb{R}^d \times \mathbb{R} \times \mathbb{R}^{N_s} &\mapsto \mathcal{D}, \\ \vec{x}, t, \vec{u}^s &\mapsto \mathcal{E}(\vec{x}, t, \vec{u}^s). \end{align*}
\pagebreak

$\mathcal{L}$
\pagebreak

\begin{align*} \mathcal{L}: \mathcal{D}_1 \times \dots \times \mathcal{D}_{n_{\mathcal{L}}} &\mapsto \mathcal{D}, \\ \mathcal{E}_1, \dots, \mathcal{E}_{n_{\mathcal{L}}} &\mapsto \mathcal{L}(\mathcal{E}_1, \dots, \mathcal{E}_{n_{\mathcal{L}}} ). \end{align*}
\pagebreak

\begin{align*} \left. \frac{\partial \mathcal{L}}{\partial \vec{u}^t} \right|_{\vec{u}} = \sum\limits_{k=1}^{n_{\mathcal{L}}} \left. \frac{\partial \mathcal{L}}{\partial \mathcal{I}_k} \right|_{\vec{u}} \cdot \left. \frac{\partial \mathcal{I}_k}{\partial \vec{u}^t} \right|_{\vec{u}} \end{align*}
\pagebreak

$ (\vec{x}, t) $
\pagebreak

$ A_{this} \leftarrow A_{this} + B$
\pagebreak

$ A_{this} \leftarrow A_{this} - B$
\pagebreak

$ \det(M M^T) $
\pagebreak

$ \sqrt{\det(M M^T)} $
\pagebreak

$ A \in \mathbb{R}^{M \times N} $
\pagebreak

$ M \leq N $
\pagebreak

\[ A^{-1}_{right} := A^T (A A^T)^{-1}, \]
\pagebreak

$ A A^{-1}_{right} = 1 $
\pagebreak

$ \det{A A^T} $
\pagebreak

$ N = M $
\pagebreak

$ M \geq N $
\pagebreak

\[ A^{-1}_{left} := (A^T A)^{-1} A^T, \]
\pagebreak

$ A^{-1}_{left} A = 1 $
\pagebreak

$ \det{A^T A} $
\pagebreak

$ A = Q R $
\pagebreak

$ Q^T = Q^{-1} $
\pagebreak

$ v \gets Q^{-1} v $
\pagebreak

$ A^{-1} $
\pagebreak

$ v := A^{-1} v $
\pagebreak

$o_i=\sqrt {v_i}$
\pagebreak

$ \vec{x} in P $
\pagebreak

\[ (\vec{x}�- \vec{r0}) \cdot \vec{n} = 0. \]
\pagebreak

$L_2$
\pagebreak

$[-1, 1]$
\pagebreak

$P_0 (x) = 1$
\pagebreak

$P_1 (1) = x$
\pagebreak

$P_k (x) = ((2 k - 1) x P_{k-1} (x) - (k - 1) P_{k-2} (x)) / k$
\pagebreak

$P_k$
\pagebreak

$\sqrt {2 / (2 k + 1)}$
\pagebreak

$k \ge 0$
\pagebreak

$2 / (2 k + 1)$
\pagebreak

$\sqrt {\frac{1}{b-a} \int_a^b P_k^2 (x) \, dx}$
\pagebreak

$a=-1$
\pagebreak

$b=1$
\pagebreak

$(n+1) P_k (x) = (2 k - 1) x P_{k-1} (x) - (k - 1) P_{n-2} (x)$
\pagebreak

$\sqrt {(2 k + 1) / 2} P_k (x)$
\pagebreak

$ \int_{-1}^1 \phi (x) \cdot \psi (x) \frac{1}{\sqrt {1 - x^2}} \, dx $
\pagebreak

$T_0 (x) = 1$
\pagebreak

$T_1 (1) = x$
\pagebreak

$T_k (x) = 2 x P_{k-1} (x) - P_{k-2} (x)$
\pagebreak

$T_k$
\pagebreak

$\tfrac{\pi}{2}$
\pagebreak

$k > 0$
\pagebreak

$\pi$
\pagebreak

$k = 0$
\pagebreak

$T_k (x) = 2 x T_{k-1} (x) - T_{k-2} (x)$
\pagebreak

$T_k (x)$
\pagebreak

$ \int_{-1}^1 \phi (x) \cdot \psi (x) \sqrt {1 - x^2} \, dx $
\pagebreak

$U_0 (x) = 1$
\pagebreak

$U_1 (1) = 2 x$
\pagebreak

$U_k (x) = 2 x U_{k-1} (x) - U_{k-2} (x)$
\pagebreak

\begin{eqnarray*} min_{x \in \mathbb{R}^n} f(x) \end{eqnarray*}
\pagebreak

\begin{eqnarray*} c_i(x) = 0, \qquad i \in E \\ c_i(x) \ge 0 \qquad i \in I, \end{eqnarray*}
\pagebreak

$ f $
\pagebreak

$ \mathbb{R}^n $
\pagebreak

$ E $
\pagebreak

$ A $
\pagebreak

\begin{eqnarray*} A(x) := E \cup \{ i \in I | c_i(x) = 0 \}, \end{eqnarray*}
\pagebreak

$ c_i(x) = 0 $
\pagebreak

$ c_i(x) > 0 $
\pagebreak

\begin{eqnarray*} a \ge 0, \, b \ge 0, \, a b = 0 \end{eqnarray*}
\pagebreak

$ a, b \in \mathbb{R}^n $
\pagebreak

\begin{eqnarray*} C(a,b) = 0, \end{eqnarray*}
\pagebreak

$ C: \mathbb{R}^n x \mathbb{R}^n \to \mathbb{R}^n $
\pagebreak

$ C $
\pagebreak

$ K u = f $
\pagebreak

$ K $
\pagebreak

$ u, f $
\pagebreak

$ \lambda $
\pagebreak

$ \lambda := f - K u $
\pagebreak

$ A = D - L - U $
\pagebreak

$ x^{m+1} = M * x^m + N * b $
\pagebreak

$ M $
\pagebreak

$ N \in R^{nxn} $
\pagebreak

$ x^{m+1} = x^m - N * (A * x^m - b) $
\pagebreak

$ c{m+1} := x^{m+1} - x^m $
\pagebreak

$ d^m := b - A * x^m $
\pagebreak

$ c = N * d $
\pagebreak

$ N = (D-L)^{-1}$
\pagebreak

$ N = (D-U)^{-1}$
\pagebreak

$ N = (D-u)^{-1}D(D-U)^{-1} $
\pagebreak

$A = D - L - U$
\pagebreak

$ c = N * d = (D-L)^{-1} * d $
\pagebreak

$c = N * d = (D-U)^{-1} * d $
\pagebreak

$A = D - L - R$
\pagebreak

$c = N * d = (D-U)^{-1} D (D-L)^{-1} d $
\pagebreak

$c = N * d = D^{-1} d $
\pagebreak

\[ M_{ij} = \sum_{kl} A_{ik} * B_{kl} * C_{lj} \]
\pagebreak

\[ M_{ij} += \sum_{kl} A_{ik} * B_{kl} * C_{lj} \]
\pagebreak

$ M_{ij} = \sum_k A_{ik} * B_{kj} $
\pagebreak

$x = (D-L)^{-1}b $
\pagebreak

$x = (D-U)^{-1}b $
\pagebreak

$x = (D-U)^{-1} D (D-L)^{-1} b $
\pagebreak

$x = D^{-1} b $
\pagebreak

$ A*x = b $
\pagebreak

\[ x = x + c, \]
\pagebreak

$ c = B*d $
\pagebreak

$ \kappa $
\pagebreak

\[ x = x + \kappa c. \]
\pagebreak

$B_{\Delta}$
\pagebreak

$u_{\Delta}$
\pagebreak

$B_{\Delta}^T$
\pagebreak

$d$
\pagebreak

$\lambda$
\pagebreak

$f_{\Delta}$
\pagebreak

$S_{\Delta}^{i}$
\pagebreak

$ \Delta $
\pagebreak

$ \Pi $
\pagebreak

${\tilde{S}_{\Delta \Delta}}^{-1}$
\pagebreak

$ A = \sum\limits_{p=1}^{N} A^{(p)}$
\pagebreak

\begin{align*} A^{(p)} \begin{pmatrix} A_{II}^{(p)} & A_{I \Delta}^{(p)} & A_{I \Pi}^{(p)} \\ A_{\Delta I}^{(p)} & A_{\Delta \Delta}^{(p)} & A_{\Delta \Pi}^{(p)} \\ A_{\Pi I}^{(p)} & A_{\Pi \Delta}^{(p)} & A_{\Pi \Pi}^{(p)} \end{pmatrix} \end{align*}
\pagebreak

\begin{align*} S_{\Delta \Delta} = A_{\Delta \Delta} - \begin{pmatrix} A_{I \Delta}^T & A_{\Pi \Delta}^T \end{pmatrix} \begin{pmatrix} A_{II} & A_{I \Pi} \\ A_{\Pi I} & A_{\Pi \Pi} \end{pmatrix}^{-1} \begin{pmatrix} A_{I \Delta} \\ A_{\Pi \Delta} \end{pmatrix} * \end{align*}
\pagebreak

$A_{II}$
\pagebreak

$\Delta$
\pagebreak

$\Pi$
\pagebreak

$F$
\pagebreak

$v$
\pagebreak

$F := B_{\Delta} \tilde{S}^{-1} B_{\Delta}^T$
\pagebreak

$d := B_{\Delta} \tilde{S}_{\Delta \Delta}^{-1} \tilde{f}_{\Delta}$
\pagebreak

$\tilde{f}_{\Delta}$
\pagebreak

$D_{\Delta}^{(i)}$
\pagebreak

$ M^{-1,(i)} $
\pagebreak

$ r $
\pagebreak

$M^{-1,(i)} := D_{\Delta}^{(i)} B_{\Delta}^{(i)} S_{\Delta}^{(i)} {B_{\Delta}^{(i)}}^T D_{\Delta}^{(i)}$
\pagebreak

$r$
\pagebreak

$ M^{-1} $
\pagebreak

$F \lambda = d$
\pagebreak

$ -a_{ij} \ge \epsilon \max_{a_{ik}<0} |a_{ik}| $
\pagebreak

$ ILU_{\beta} $
\pagebreak

$ N = D^{-1} $
\pagebreak

$ f_{\Gamma} = (A_{\Gamma, \Gamma} - A_{\Gamma, I} A_{I, I}^{-1} A_{I, \Gamma} )u_{\Gamma} $
\pagebreak

\begin{eqnarray*} A = T_L^{-1} \hat{A} T_R \end{eqnarray*}
\pagebreak

\begin{eqnarray*} x := x + T_R^{-1} {\hat{A}}^{-1} T_L (b-Ax) \end{eqnarray*}
\pagebreak

$ \partial_t u + A(u) = f $
\pagebreak

\[ d(u^k) = \sum_{i=0}^{l-1} s_{m,i} M(u^{k-i}) + s_{a,i} \{A(u^{k-i}) - f\} \]
\pagebreak

$ \partial_t u + A*u = f $
\pagebreak

\[ d(u^k) = \sum_{i=0}^{l-1} s_{m,i} M*u^{k-i} + s_{a,i} \{A*u^{k-i} - f \} J(u^k) = s_{m,0}*M + s_{a,0} A \]
\pagebreak

$ A = s_{m,0}*M + s_{a,0} A $
\pagebreak

$ b = - \{ \sum_{i=1}^{l-1} s_{m,i} M*u^{k-i} + s_{a,i} \{A*u^{k-i} - f\} \} + s_{a,0} * f $
\pagebreak

$ A(u) = f $
\pagebreak

\[ d(u) = A(u) - f \]
\pagebreak

$ A*u = f $
\pagebreak

\[ d(u) = A*u - f J(u) = A \]
\pagebreak

$ A = A $
\pagebreak

$ b = f $
\pagebreak

$ \theta * (\mu + width * \sigma) $
\pagebreak

$ \mu = E[\eta^2], \sigma^2 = Var[\eta^2] $
\pagebreak

$ \mu = E[\eta], \sigma^2 = Var[\eta] $
\pagebreak

$ \eta_i^2 $
\pagebreak

$\rho$
\pagebreak

$\rho(u)$
\pagebreak

$f$
\pagebreak

$f^2(u)$
\pagebreak

$u_1$
\pagebreak

$u_2$
\pagebreak

$ (f(u_1)- f(u_2))^2 $
\pagebreak

$ \| q \|^2 $
\pagebreak

$ q:= \kappa \nabla u $
\pagebreak

$ |D \nabla u|^2 $
\pagebreak

$ -c \cdot \vec{n} $
\pagebreak

$ - \nabla c \cdot \vec{n} $
\pagebreak

\[ \prod_{j=0}^{i-1} \frac{x - \frac{j}{p}}{\frac{i}{p} - \frac{j}{p}} \]
\pagebreak

\[ \prod_{\substack{j=0\\j\neq i}}^{b} \frac{x - \frac{j}{p}}{\frac{i}{p} - \frac{j}{p}} \]
\pagebreak

$ \{ K, P, \Sigma \} $
\pagebreak

$\mathbb{R}^d$
\pagebreak

$ P $
\pagebreak

$p: K \mapsto \mathbb{R}^m $
\pagebreak

$m > 0 $
\pagebreak

$m=1$
\pagebreak

$m=d$
\pagebreak

$\Sigma$
\pagebreak

$ n_{sh} $
\pagebreak

$ \sigma_1, \dots, \sigma_{n_{sh}} $
\pagebreak

\[ p \mapsto ( \sigma_1(p), \dots, \sigma_{n_{sh}}(p)) \in \mathbb{R}^{n_{sh}} \]
\pagebreak

$\{\phi_1, \dots, \phi_{n_{sh}} \subset P$
\pagebreak

\[ \sigma_i (\phi_j) = \delta_{ij}, \qquad 1 \leq i,j \leq n_{sh}. \]
\pagebreak

\[ \int\limits_T f(\mathbf{x}) \; d\mathbf{x} \approx \sum_{i=0}^{n-1} f(\mathbf{x}_{i}) \cdot w_i \]
\pagebreak

$n$
\pagebreak

$\mathbf{x}_i$
\pagebreak

$ w_i $
\pagebreak

$R$
\pagebreak

$T$
\pagebreak

\[ \phi: R \mapsto T \]
\pagebreak

$\mathbf{v} = \mathbf{K} (- \nabla p + \rho \mathbf{g}) / \mu$
\pagebreak

$\mathbf{K}$
\pagebreak

$\mu$
\pagebreak

$\mathbf{g}$
\pagebreak

$p$
\pagebreak

$rho$
\pagebreak

$\nabla p$
\pagebreak

$\rho \mathbf{g}$
\pagebreak

$\mathbf{h} = (h_x, h_y, \dots)$
\pagebreak

$\mathbf{v} = - \mathbf{K} (p_x - h_x, p_y - h_y, \dots) / \mu$
\pagebreak

$\mathbf{h}$
\pagebreak

$h$
\pagebreak

\[ \nabla \cdot (\mathbf{v} c) \]
\pagebreak

$\mathbf{v}$
\pagebreak

$ip$
\pagebreak

\[ \sum_{s=1}^{n_s} \phi_s (ip) \, c_s, \]
\pagebreak

$\phi_s (ip)$
\pagebreak

$n_s$
\pagebreak

$c$
\pagebreak

$ \mathbf{x}_i $
\pagebreak

$ u_i $
\pagebreak

$ u $
\pagebreak

$ \mathbf{x} \not\in \{ \mathbf{x}_i \} $
\pagebreak

\begin{eqnarray*} u = \frac {\sum_i w_i \cdot u_i} {\sum_i w_i}, \end{eqnarray*}
\pagebreak

\begin{eqnarray*} w_i := \frac{1}{\| \mathbf{x} - \mathbf{x}_i \|_2^p} \end{eqnarray*}
\pagebreak

$ p $
\pagebreak

$ \mathbf{x} = \mathbf{x}_i $
\pagebreak

$ u = u_i $
\pagebreak

$ \mathbf{x} $
\pagebreak

$ R $
\pagebreak

$ \| \mathbf{x} - \mathbf{x}_i \|_2 \le R $
\pagebreak

$ S $
\pagebreak

$ \Omega $
\pagebreak

$ 1 $
\pagebreak

$ \Omega \setminus S $
\pagebreak

$ \mathbf{q} = - \frac{\mathbf{K}}{\mu} ( \nabla p - \rho \mathbf{g} ) $
\pagebreak

$ \mathbf{K} $
\pagebreak

$ \mu $
\pagebreak

$ \rho $
\pagebreak

$ \mathbf{g} $
\pagebreak

$ \nabla p $
\pagebreak

\[ \partial_t u(t) = f(t) \]
\pagebreak

\[ \frac{u(t^{k+1}) - u(t^k)}{\Delta t} = (1-\theta) \cdot f(t^{k+1}) + \theta \cdot f(t^k) \]
\pagebreak

$\theta = 1 $
\pagebreak

\end{document}
